pulse/src/syntax_extension/PulseSyntaxExtension.Sugar.fst
@@ -172,7 +172,7 @@ and lambda = {
   range:rng
 }
 
-and fn_decl = {
+and fn_defn = {
   id:ident;
   is_rec:bool;
   binders:binders;
@@ -185,7 +185,7 @@ and fn_decl = {
 and let_init =
   | Array_initializer of array_init
   | Default_initializer of A.term
-  | Lambda_initializer of fn_decl
+  | Lambda_initializer of fn_defn
   | Stmt_initializer of stmt
 
 let tag_of_stmt (s:stmt) : string =
@@ -206,7 +206,7 @@ let tag_of_stmt (s:stmt) : string =
   | WithInvariants {} -> "WithInvariants"
 
 type decl =
-  | FnDecl of fn_decl
+  | FnDefn of fn_defn
   
 (* Convenience builders for use from OCaml/Menhir, since field names get mangled in OCaml *)
 let mk_comp tag precondition return_name return_type postcondition opens range = 
@@ -232,7 +232,7 @@ let mk_while guard id invariant body = While { guard; id; invariant; body }
 let mk_intro vprop witnesses = Introduce { vprop; witnesses }
 let mk_sequence s1 s2 = Sequence { s1; s2 }
 let mk_stmt s range = { s; range }
-let mk_fn_decl id is_rec binders ascription measure body range = { id; is_rec; binders; ascription; measure; body; range }
+let mk_fn_defn id is_rec binders ascription measure body range = { id; is_rec; binders; ascription; measure; body; range }
 let mk_open lid = Open lid
 let mk_par p1 p2 q1 q2 b1 b2 = Parallel { p1; p2; q1; q2; b1; b2 }
 let mk_proof_hint_with_binders ht bs =  ProofHintWithBinders { hint_type=ht; binders=bs }
